{-# OPTIONS --without-K #-}

open import Agda.Primitive
open import Base
open import Equality
open import Homotopies
open import Composition
open import EquationalReasoning
open import logic.Contractible
open import logic.Propositions
open import equality.Sigma
open import equivalence.Equivalence

module equivalence.Halfadjoints {ℓᵢ ℓⱼ} {A : Type ℓᵢ} {B : Type ℓⱼ} where

  -- Half adjoint equivalence
  record ishae (f : A → B) : Type (ℓᵢ ⊔ ℓⱼ) where
    constructor hae
    field
      g : B → A
      η : (g ∘ f) ∼ id
      ε : (f ∘ g) ∼ id
      τ : (x : A) → ap f (η x) == ε (f x)
    
  -- Half adjoint equivalences give contractible fibers
  ishae-contr : (f : A → B) → ishae f → isContrMap f
  ishae-contr f (hae g η ε τ) y = ((g y) , (ε y)) , contra
    where
      lemma : (c c' : fib f y) → Σ (fst c == fst c') (λ γ → (ap f γ) · snd c' == snd c) → c == c'
      lemma c c' (p , q) = Σ-bycomponents (p , lemma2)
        where
          lemma2 : transport (λ z → f z == y) p (snd c) == snd c'
          lemma2 = 
            begin
              transport (λ z → f z == y) p (snd c)   ==⟨ transport-eq-fun-l f p (snd c) ⟩
              inv (ap f p) · (snd c)                 ==⟨ ap (inv (ap f p) ·_) (inv q) ⟩
              inv (ap f p) · ((ap f p) · (snd c'))   ==⟨ inv (·-assoc (inv (ap f p)) (ap f p) (snd c')) ⟩
              inv (ap f p) · (ap f p) · (snd c')     ==⟨ ap (_· (snd c')) (·-linv (ap f p)) ⟩
              snd c'
            ∎
            
      contra : (x : fib f y) → (g y , ε y) == x
      contra (x , p) = lemma (g y , ε y) (x , p) (γ , lemma3)
        where
          γ : g y == x
          γ = inv (ap g p) · η x
      
          lemma3 : (ap f γ · p) == ε y
          lemma3 =
            begin
              ap f γ · p                                 ==⟨ ap (_· p) (ap-· f (inv (ap g p)) (η x)) ⟩
              ap f (inv (ap g p)) · ap f (η x) · p       ==⟨ ·-assoc (ap f (inv (ap g p))) _ p ⟩
              ap f (inv (ap g p)) · (ap f (η x) · p)     ==⟨ ap (_· (ap f (η x) · p)) (ap-inv f (ap g p)) ⟩
              inv (ap f (ap g p)) · (ap f (η x) · p)     ==⟨ ap (λ u → inv (ap f (ap g p)) · (u · p)) (τ x) ⟩
              inv (ap f (ap g p)) · (ε (f x) · p)        ==⟨ ap (λ u → inv (ap f (ap g p)) · (ε (f x) · u))
                                                             (inv (ap-id p)) ⟩
              inv (ap f (ap g p)) · (ε (f x) · ap id p)  ==⟨ ap (inv (ap f (ap g p)) ·_) (h-naturality ε p) ⟩
              inv (ap f (ap g p)) · (ap (f ∘ g) p · ε y)  ==⟨ ap (λ u → inv u · (ap (f ∘ g) p · ε y))
                                                             (ap-comp g f p) ⟩
              inv (ap (f ∘ g) p) · (ap (f ∘ g) p · ε y)   ==⟨ inv (·-assoc (inv (ap (f ∘ g) p)) _ (ε y)) ⟩
              (inv (ap (f ∘ g) p) · ap (f ∘ g) p) · ε y   ==⟨ ap (_· ε y) (·-linv (ap (λ z → f (g z)) p)) ⟩
              ε y
            ∎

  ishae-≃ : {f : A → B} → ishae f → A ≃ B
  ishae-≃ ishaef = _ , (ishae-contr _ ishaef)

